---
prev: false
next: false
---

<script setup>
import { VPButton } from 'vitepress/theme';
</script>

**Самостоятельная работа**

# Самостоятельная работа №1

Найти общее решение уравнения с частными производными.

<a href="/media/files/kp1_PDE1_R.pdf" target="_blank"><VPButton text="Скачать PDF" theme="alt" style="padding: 0 12px; line-height: 2; float: right; transform: translateY(3.55rem)" /></a>
## Варианты

| № | Уравнение |
|-|-|
| 1 | $\displaystyle (3x + 5y) ~ {\partial z \over \partial x} + (-5x + 3y) ~ {\partial z \over \partial y} = 0$ |
| 2 | $\displaystyle (-4x - 25y) ~ {\partial z \over \partial x} + (x + 4y) ~ {\partial z \over \partial y} = 0$ |
| 3 | $\displaystyle (-2x + 5y) ~ {\partial z \over \partial x} + (-5x - 2y) ~ {\partial z \over \partial y} = 0$ |
| 4 | $\displaystyle (x - y) ~ {\partial z \over \partial x} + (17x - y) ~ {\partial z \over \partial y} = 0$ |
| 5 | $\displaystyle (x + 3y) ~ {\partial z \over \partial x} + (-6x - 5y) ~ {\partial z \over \partial y} = 0$ |
| 6 | $\displaystyle (2x + 3y) ~ {\partial z \over \partial x} + (-3x + 2y) ~ {\partial z \over \partial y} = 0$ |
| 7 | $\displaystyle (x - y) ~ {\partial z \over \partial x} + (2x - y) ~ {\partial z \over \partial y} = 0$ |
| 8 | $\displaystyle (2x + 3y) ~ {\partial z \over \partial x} + 5x ~ {\partial z \over \partial y} = 0$ |
| 9 | $\displaystyle 3y ~ {\partial z \over \partial x} + (7x + 4y) ~ {\partial z \over \partial y} = 0$ |
| 10 | $\displaystyle (2x + 15y) ~ {\partial z \over \partial x} + x ~ {\partial z \over \partial y} = 0$ |
| 11 | $\displaystyle y ~ {\partial z \over \partial x} + (8x + 2y) ~ {\partial z \over \partial y} = 0$ |
| 12 | $\displaystyle x ~ {\partial z \over \partial x} + (2x - y) ~ {\partial z \over \partial y} = 0$ |
| 13 | $\displaystyle (-2x + 3y) ~ {\partial z \over \partial x} + (4x + 2y) ~ {\partial z \over \partial y} = 0$ |
| 14 | $\displaystyle (3x - 2y) ~ {\partial z \over \partial x} + (-6x + 4y) ~ {\partial z \over \partial y} = 0$ |
| 15 | $\displaystyle (-2x + 5y) ~ {\partial z \over \partial x} + (-5x - 2y) ~ {\partial z \over \partial y} = 0$ |
| 16 | $\displaystyle (-2x + 8y) ~ {\partial z \over \partial x} + (-x + 2y) ~ {\partial z \over \partial y} = 0$ |
| 17 | $\displaystyle (3x - y) ~ {\partial z \over \partial x} + (x + 3y) ~ {\partial z \over \partial y} = 0$ |
| 18 | $\displaystyle (x - 5y) ~ {\partial z \over \partial x} + (2x - y) ~ {\partial z \over \partial y} = 0$ |
| 19 | $\displaystyle (x + 2y) ~ {\partial z \over \partial x} + (-2x + y) ~ {\partial z \over \partial y} = 0$ |
| 20 | $\displaystyle (4x - 5y) ~ {\partial z \over \partial x} + x ~ {\partial z \over \partial y} = 0$ |
| 21 | $\displaystyle 3y ~ {\partial z \over \partial x} + (7x - 4y) ~ {\partial z \over \partial y} = 0$ |
| 22 | $\displaystyle (-2x + 3y) ~ {\partial z \over \partial x} + 5x ~ {\partial z \over \partial y} = 0$ |
| 23 | $\displaystyle 4y ~ {\partial z \over \partial x} + (3x + 4y) ~ {\partial z \over \partial y} = 0$ |
| 24 | $\displaystyle (2x + y) ~ {\partial z \over \partial x} + 15x ~ {\partial z \over \partial y} = 0$ |
| 25 | $\displaystyle 2y ~ {\partial z \over \partial x} + (6x + 4y) ~ {\partial z \over \partial y} = 0$ |
| 26 | $\displaystyle 3y ~ {\partial z \over \partial x} + (7x - 4y) ~ {\partial z \over \partial y} = 0$ |
| 27 | $\displaystyle (-2x + 3y) ~ {\partial z \over \partial x} + 5x ~ {\partial z \over \partial y} = 0$ |
| 28 | $\displaystyle 4y ~ {\partial z \over \partial x} + (3x + 4y) ~ {\partial z \over \partial y} = 0$ |
| 29 | $\displaystyle (2x + y) ~ {\partial z \over \partial x} + 15x ~ {\partial z \over \partial y} = 0$ |
| 30 | $\displaystyle 2y ~ {\partial z \over \partial x} + (6x + 4y) ~ {\partial z \over \partial y} = 0$ |
| 31 | $\displaystyle (x - y) ~ {\partial z \over \partial x} + (17x - y) ~ {\partial z \over \partial y} = 0$ |
